Use share and call in examples #183

base/coq/Free/Verification/SharingHandlerTests.v
@@ -46,32 +46,51 @@ Section SecData.
   Notation "'ND'" := (Injectable ND.Shape ND.Pos Shape Pos).
   Notation "'Trace'" := (Traceable Shape Pos).
   Notation "'Maybe'" := (Injectable Maybe.Shape Maybe.Pos Shape Pos).
+  Notation "'Share'" := (Injectable Share.Shape Share.Pos Shape Pos).
 
   (* Non-deterministic integer. *)
-  Definition coin `{ND}
-  := Choice Shape Pos (pure 0%Z) (pure 1%Z).
+  Definition coin `{ND} `{I : Share} (S : Strategy Shape Pos)
+  := @call Shape Pos I S _ (pure 0%Z) >>= fun c1 =>
+     @call Shape Pos I S _ (pure 1%Z) >>= fun c2 =>
+     Choice Shape Pos c1 c2.
 
   (* Non-deterministic boolean value. *)
-  Definition coinB `{ND} := Choice Shape Pos (True_ _ _) (False_ _ _).
+  Definition coinB `{ND} `{I : Share} (S : Strategy Shape Pos)
+  := @call Shape Pos I S _ (True_ Shape Pos) >>= fun c1 =>
+     @call Shape Pos I S _ (False_ Shape Pos) >>= fun c2 =>
+     Choice Shape Pos c1 c2.
 
   (* Non-deterministic partial integer. *)
-  Definition coinM `{ND} `{Maybe} 
-  := Choice Shape Pos (Nothing_inj _ _) (Just_inj _ _ 1%Z).
+  Definition coinM `{ND} `{Maybe} `{I : Share} (S : Strategy Shape Pos)
+  := @call Shape Pos I S _ (Nothing_inj Shape Pos) >>= fun c1 =>
+     @call Shape Pos I S _ (Just_inj Shape Pos 1%Z) >>= fun c2 =>
+     Choice Shape Pos c1 c2.
 
   (* (0 ? 1, 2 ? 3) *)
-  Definition coinPair `{ND}
+  Definition coinPair `{ND} `{I : Share} (S : Strategy Shape Pos)
   : Free Shape Pos (Pair Shape Pos (Integer Shape Pos) (Integer Shape Pos))
-  := Pair_ Shape Pos (Choice Shape Pos (pure 0%Z) (pure 1%Z))
-                     (Choice Shape Pos (pure 2%Z) (pure 3%Z)).
+  := @call Shape Pos I S _ (pure 0%Z) >>= fun c1 =>
+     @call Shape Pos I S _ (pure 1%Z) >>= fun c2 =>
+     @call Shape Pos I S (Integer Shape Pos) 
+          (Choice Shape Pos c1 c2) >>= fun c3 =>
+     @call Shape Pos I S _ (pure 2%Z) >>= fun c4 =>
+     @call Shape Pos I S _ (pure 3%Z) >>= fun c5 =>
+     @call Shape Pos I S (Integer Shape Pos) 
+          (Choice Shape Pos c4 c5) >>= fun c6 =>
+     Pair_ Shape Pos c3 c6.
 
   (* [0 ? 1, 2 ? 3] *)
-  Definition coinList `{ND}
+  Definition coinList `{ND} `{I : Share} (S : Strategy Shape Pos)
   : Free Shape Pos (List Shape Pos (Integer Shape Pos))
-  := List.Cons Shape Pos 
-       (Choice Shape Pos (pure 0%Z) (pure 1%Z))
-       (List.Cons Shape Pos 
-         (Choice Shape Pos (pure 2%Z) (pure 3%Z))
-         (List.Nil Shape Pos)).
+  := @call Shape Pos I S _ (List.Nil Shape Pos) >>= fun c1 =>
+     @call Shape Pos I S _ (pure 2%Z) >>= fun c2 =>
+     @call Shape Pos I S _ (pure 3%Z) >>= fun c3 =>
+     @call Shape Pos I S _ (Choice Shape Pos c2 c3) >>= fun c4 =>
+     @call Shape Pos I S _ (List.Cons Shape Pos c2 c1) >>= fun c5 => 
+     @call Shape Pos I S _ (pure 0%Z) >>= fun c6 =>
+     @call Shape Pos I S _ (pure 1%Z) >>= fun c7 =>
+     @call Shape Pos I S _ (Choice Shape Pos c6 c7) >>= fun c8 =>
+     List.Cons Shape Pos c8 c5.
 
 
   (* Traced integer. *)
@@ -106,11 +125,11 @@ Section SecData.
 End SecData.
 
 (* Arguments sentences for the data. *)
-Arguments coin {_} {_} {_}.
-Arguments coinB {_} {_} {_}.
-Arguments coinM {_} {_} {_} {_}.
-Arguments coinPair {_} {_} {_}.
-Arguments coinList {_} {_} {_}.
+Arguments coin {_} {_} {_} {_} _.
+Arguments coinB {_} {_} {_} {_} _.
+Arguments coinM {_} {_} {_} {_} {_} _.
+Arguments coinPair {_} {_} {_} {_} _.
+Arguments coinList {_} {_} {_} {_} _.
 Arguments traceOne {_} {_} {_}.
 Arguments traceTrue {_} {_} {_}.
 Arguments traceFalse {_} {_} {_}.
@@ -147,7 +166,8 @@ Section SecFunctions.
                                 (f : FreeA -> FreeA -> FreeA)
                                 (fx : FreeA)
    : FreeA
-  := @share Shape Pos I S A SA (@share Shape Pos I S A SA fx >>= fun sx => f sx sx) >>= fun sy =>
+  := @share Shape Pos I S A SA fx >>= fun sx => 
+     @share Shape Pos I S A SA (f sx sx) >>= fun sy =>
     f sy sy.
 
   (* let sx = fx  
@@ -158,38 +178,64 @@ Section SecFunctions.
                               (f : FreeA -> FreeA -> FreeA)
                               (fx : FreeA) (fy : FreeA)
   : FreeA
-  := @share Shape Pos I S A SA (@share Shape Pos I S A SA fx >>= fun sx => f sx sx) >>= fun sy =>
-    @share Shape Pos I S A SA fy >>=  fun sz => f sy sz.
+  := @share Shape Pos I S A SA fx >>= fun sx =>
+     @call Shape Pos I S A (f sx sx) >>= fun sy =>
+     @call Shape Pos I S A fy >>= fun sz => 
+     f sy sz.
 
   (*
   let sx = val
      sy = f sx fx
      sz = f sy fy
-  in f sx (f sy (f sz val)) 
+     c1 = f sz val
+     c2 = f sy c1
+  in f sx c2
   *)
   Definition doubleSharedRec `{I : Share} `{SA : ShareArgs} (S : Strategy Shape Pos)
                              (f : FreeA -> FreeA -> FreeA)
                             (fx : FreeA) (fy : FreeA)
                             (val : A)
    : FreeA
-  := @share Shape Pos I S A SA (pure val) >>= fun sx =>
-    f sx (@share Shape Pos I S A SA (f sx fx) >>= fun sy => 
-    f sy (@share Shape Pos I S A SA (f sy fy) >>= fun sz =>
-    f sz (pure val))).
+  := @call Shape Pos I S A (pure val) >>= fun sx =>
+     @share Shape Pos I S A SA (f sx fx) >>= fun sy =>
+     @share Shape Pos I S A SA (f sy fy) >>= fun sz =>
+     @call Shape Pos I S A (f sz sx) >>= fun c1 =>
+     @call Shape Pos I S A (f sy c1) >>= fun c2 =>
+     f sx c2.
 
   (* Deep sharing. *)
+
+  (* 
+  let sx = fx
+      c1 = fst sx
+      c2 = fst sx
+      in c1 + c2
+  *)
   Definition doubleDeepSharedPair `{I : Share} `{SA : ShareArgs} (S : Strategy Shape Pos)
                         (f : FreeA -> FreeA -> FreeA)
                         (fx : Free Shape Pos (Pair Shape Pos A A))
    : FreeA
-  := @share Shape Pos I S (Pair Shape Pos A A) _ fx >>= fun sx => f (fstPair Shape Pos sx) (fstPair Shape Pos sx).
+  := @share Shape Pos I S (Pair Shape Pos A A) _ fx >>= fun sx => 
+     @call Shape Pos I S A (fstPair Shape Pos sx) >>= fun c1 =>
+     @call Shape Pos I S A (fstPair Shape Pos sx) >>= fun c2 =>
+      f c1 c2.
 
+  (* 
+  let sx = fl in head sx + head sx
+  Flattened version:
+  let sx = fl
+      c1 = head sx
+      c2 = head sx
+  in c1 + c2
+  *)
   Definition doubleDeepSharedList `{I : Share} `{SA : ShareArgs} (P : Partial Shape Pos) (S : Strategy Shape Pos)
                         (f : FreeA -> FreeA -> FreeA)
                         (fl : Free Shape Pos (List Shape Pos A))
    : FreeA
-  := @share Shape Pos I S (List Shape Pos A) _ fl >>= fun sx => 
-              f (headList Shape Pos P sx) (headList Shape Pos P sx).
+  := @share Shape Pos I S (List Shape Pos A) _ fl >>= fun sx =>
+     @call Shape Pos I S A (headList Shape Pos P sx) >>= fun c1 =>
+     @call Shape Pos I S A (headList Shape Pos P sx) >>= fun c2 =>
+              f c1 c2.
 
 End SecFunctions.
 
@@ -209,7 +255,7 @@ Notation "'orBool_'" := (orBool _ _).
 = 0+0 ? 0+1 ? 1+0 ? 1+1
 = 0 ? 1 ? 1 ? 2
 *)
-Example exAddNoSharingND : evalND (nf (doubleShared  Cbn_ addInteger_ coin))
+Example exAddNoSharingND : evalND (nf (doubleShared  Cbn_ addInteger_ (coin Cbn_)))
                            = [0%Z;1%Z;1%Z;2%Z].
 Proof. constructor. Qed.
 
@@ -229,7 +275,7 @@ Proof. constructor. Qed.
 = true ? true ? false
 *)
 Example exOrNDNoSharing 
- : evalND (nf (doubleShared Cbn_ orBool_ coinB)) = [true;true;false].
+ : evalND (nf (doubleShared Cbn_ orBool_ (coinB Cbn_))) = [true;true;false].
 Proof. constructor. Qed.
 
 (*
@@ -270,7 +316,7 @@ Proof. constructor. Qed.
 = Nothing ? Nothing ? Just 2
 *)
 Example exNDMNoSharing
- : evalNDM (nf (doubleShared Cbn_ addInteger_ coinM)) = [None;None;Some 2%Z].
+ : evalNDM (nf (doubleShared Cbn_ addInteger_ (coinM Cbn_))) = [None;None;Some 2%Z].
 Proof. constructor. Qed.
 
 (* 
@@ -303,7 +349,7 @@ in sx + sx
 = 0 ? 2
 *)
 Example exAddSharingND : evalND (nf (doubleShared Cbneed_
-  addInteger_ coin))
+  addInteger_ (coin Cbneed_)))
   = [0%Z;2%Z].
 Proof. constructor. Qed.
 
@@ -324,7 +370,7 @@ in sx or sx
 = true ? false
 *)
 Example exOrNDSharing
- : evalND (nf (doubleShared Cbneed_ orBool_ coinB)) = [true;false].
+ : evalND (nf (doubleShared Cbneed_ orBool_ (coinB Cbneed_))) = [true;false].
 Proof. constructor. Qed.
 
 (*
@@ -364,7 +410,7 @@ in sx + sx
 = Nothing ? Just 2
 *)
 Example exNDMSharing
- : evalNDM (nf (doubleShared Cbneed_ addInteger_ coinM))
+ : evalNDM (nf (doubleShared Cbneed_ addInteger_ (coinM Cbneed_)))
    = [None;Some 2%Z].
 Proof. constructor. Qed.
 
@@ -401,7 +447,7 @@ in sy + sy
 *)
 Example exAddNestedSharingND : evalND (nf (doubleSharedNested Cbneed_
                                                           addInteger_ 
-                                                          coin))
+                                                          (coin Cbneed_)))
                                = [0%Z;4%Z].
 Proof. constructor. Qed.
 
@@ -423,7 +469,7 @@ in sy or sy
 = true ? false
 *)
 Example exOrNestedSharingND
- : evalND (nf (doubleSharedNested Cbneed_ orBool_ coinB))
+ : evalND (nf (doubleSharedNested Cbneed_ orBool_ (coinB Cbneed_)))
    = [true;false].
 Proof. constructor. Qed.
 
@@ -462,7 +508,7 @@ in sy + sz
 = 0 ? 1 ? 2 ? 3
 *)
 Example exAddClashSharingND
- : evalND (nf (doubleSharedClash Cbneed_ addInteger_ coin coin))
+ : evalND (nf (doubleSharedClash Cbneed_ addInteger_ (coin Cbneed_) (coin Cbneed_)))
    = [0%Z;1%Z;2%Z;3%Z].
 Proof. constructor. Qed.
 
@@ -489,7 +535,7 @@ in sy or sz
 = true ? true ? false
 *)
 Example exOrClashSharingND
- : evalND (nf (doubleSharedClash Cbneed_ orBool_ coinB coinB))
+ : evalND (nf (doubleSharedClash Cbneed_ orBool_ (coinB Cbneed_) (coinB Cbneed_)))
    = [true;true;false].
 Proof. constructor. Qed.
 
@@ -536,7 +582,7 @@ in sx + (sy + (sz + 1))
 *)
 Example exAddRecSharingND : evalND (nf (doubleSharedRec Cbneed_
                                                     addInteger_
-                                                    coin coin 1%Z))
+                                                    (coin Cbneed_) (coin Cbneed_) 1%Z))
                             = [4%Z;5%Z;6%Z;7%Z].
 Proof. constructor. Qed.
 
@@ -564,7 +610,7 @@ in sx or (sy or (sz or true))
 = true (due to non-strictness)
 *)
 Example exOrRecSharingNDTrue
- : evalND (nf (doubleSharedRec Cbneed_ orBool_ coinB coinB true))
+ : evalND (nf (doubleSharedRec Cbneed_ orBool_ (coinB Cbneed_) (coinB Cbneed_) true))
    = [true].
 Proof. constructor. Qed.
 
@@ -587,7 +633,7 @@ in sx or (sy or (sz or false))
 = true ? true ? false
 *)
 Example exOrRecSharingNDFalse
- : evalND (nf ((doubleSharedRec Cbneed_ orBool_ coinB coinB false)))
+ : evalND (nf ((doubleSharedRec Cbneed_ orBool_ (coinB Cbneed_) (coinB Cbneed_) false)))
    = [true;true;false].
 Proof. constructor. Qed.
 
@@ -631,7 +677,7 @@ in fst sx + fst sx
 = 0 ? 2
 *)
 Example exAddDeepPairND 
- : evalND (nf (doubleDeepSharedPair Cbneed_ addInteger_ coinPair))
+ : evalND (nf (doubleDeepSharedPair Cbneed_ addInteger_ (coinPair Cbneed_)))
   = [0%Z;2%Z].
 Proof. constructor. Qed.
 
@@ -642,7 +688,8 @@ in head sx + head sx
 *)
 Example exAddDeepListND
  : evalND (nf 
-  (doubleDeepSharedList (PartialLifted ND.Shape ND.Pos _ _ ND.Partial) Cbneed_ addInteger_ coinList))
+  (doubleDeepSharedList (PartialLifted ND.Shape ND.Pos _ _ ND.Partial) 
+   Cbneed_ addInteger_ (coinList Cbneed_)))
  = [0%Z;2%Z].
 Proof. constructor. Qed.
 
